wip on FunctionMemory, which requires proving that addresses do not overlap, which might be simpler with on nat than on word, therefore continue with ListMemory

src/ListMemory.v
@@ -9,36 +9,32 @@ Require Import riscv.util.Monads.
 Require Import riscv.Memory.
 Import ListNotations.
 
-Local Open Scope Z_scope.
 
 Section Memory.
-
-  Context {w: nat}. (* bit width of memory addresses *)
 
   Definition mem := list (word 8).
   Definition mem_size(m: mem): nat := length m.
 
-  Definition read_byte(m: mem)(a: word w): word 8 := nth (wordToNat a) m $0.
-  Definition read_half(m: mem)(a: word w): word 16 :=
-    let v0 := read_byte m a in let v1 := read_byte m (a ^+ $1) in combine v0 v1.
-  Definition read_word(m: mem)(a: word w): word 32 :=
-    let v0 := read_half m a in let v1 := read_half m (a ^+ $2) in combine v0 v1.
-  Definition read_double(m: mem)(a: word w): word 64 :=
-    let v0 := read_word m a in let v1 := read_word m (a ^+ $4) in combine v0 v1.
+  Definition read_byte(m: mem)(a: nat): word 8 := nth a m $0.
+  Definition write_byte(m: mem)(a: nat)(v: word 8): mem :=
+    (firstn a m) ++ [v] ++ (skipn (S a) m).
+
+  Definition read_half(m: mem)(a: nat): word 16 :=
+    let v0 := read_byte m a in let v1 := read_byte m (a + 1) in combine v0 v1.
+  Definition read_word(m: mem)(a: nat): word 32 :=
+    let v0 := read_half m a in let v1 := read_half m (a + 2) in combine v0 v1.
+  Definition read_double(m: mem)(a: nat): word 64 :=
+    let v0 := read_word m a in let v1 := read_word m (a + 4) in combine v0 v1.
 
   Definition lobits(sz: nat)(w: word (sz + sz)): word sz := split1 sz sz w.
   Definition hibits(sz: nat)(w: word (sz + sz)): word sz := split2 sz sz w.
 
-  Definition write_byte(m: mem)(a: word w)(v: word 8): mem :=
-    let i := wordToNat a in
-    (firstn i m) ++ [v] ++ (skipn (S i) m).
-
-  Definition write_half(m: mem)(a: word w)(v: word 16): mem :=
-    let m := write_byte m a (lobits 8 v) in write_byte m (a ^+ $1) (hibits 8 v).
-  Definition write_word(m: mem)(a: word w)(v: word 32): mem :=
-    let m := write_half m a (lobits 16 v) in write_half m (a ^+ $2) (hibits 16 v).
-  Definition write_double(m: mem)(a: word w)(v: word 64): mem :=
-    let m := write_word m a (lobits 32 v) in write_word m (a ^+ $4) (hibits 32 v).
+  Definition write_half(m: mem)(a: nat)(v: word 16): mem :=
+    let m := write_byte m a (lobits 8 v) in write_byte m (a + 1) (hibits 8 v).
+  Definition write_word(m: mem)(a: nat)(v: word 32): mem :=
+    let m := write_half m a (lobits 16 v) in write_half m (a + 2) (hibits 16 v).
+  Definition write_double(m: mem)(a: nat)(v: word 64): mem :=
+    let m := write_word m a (lobits 32 v) in write_word m (a + 4) (hibits 32 v).
 
   Fixpoint const_mem(default: word 8)(size: nat): mem :=
     match size with
@@ -53,7 +49,7 @@ End Memory.
 Arguments mem : clear implicits.
 
 
-Instance mem_is_Memory(w: nat): Memory mem (word w) := {|
+Instance mem_is_Memory(w: nat): Memory mem (nat) := {|
   loadByte    := read_byte;
   loadHalf    := read_half;
   loadWord    := read_word;
@@ -64,26 +60,67 @@ Instance mem_is_Memory(w: nat): Memory mem (word w) := {|
   storeDouble := write_double;
 |}.
 
-Lemma write_read_byte: forall sz m (a: word sz) v ,
-  read_byte (write_byte m a v) a = v.
+Lemma write_read_byte_eq: forall m a1 a2 v,
+    a1 < mem_size m ->
+    a2 = a1 ->
+    read_byte (write_byte m a1 v) a2 = v.
 Proof.
-  intros. unfold write_byte, read_byte in *.
-Admitted.
+  intros. subst. unfold write_byte, read_byte, mem_size in *.
+  pose proof (@firstn_length_le _ m a1).
+  rewrite app_nth2 by omega.
+  rewrite H0 by omega.
+  replace (a1 - a1) with 0 by omega.
+  reflexivity.
+Qed.
 
-Lemma write_read_byte_diff: forall sz (a1 a2: word sz) m v,
-  a2 <> a1 ->
-  read_byte (write_byte m a2 v) a1 = read_byte m a1.
+Lemma write_read_byte_ne: forall m a1 a2 v,
+    a1 < mem_size m ->
+    a2 < mem_size m ->
+    a2 <> a1 ->
+    read_byte (write_byte m a1 v) a2 = read_byte m a2.
 Proof.
-  intros. unfold read_byte, write_byte in *.
-Admitted.
+  intros. unfold write_byte, read_byte, mem_size in *.
+  pose proof (@firstn_length_le _ m a1).
+  pose proof (@firstn_length_le _ m a2).
+  assert (a2 < a1 \/ a1 < a2 < length m) as P by omega.
+  destruct P as [P | P].
+  - rewrite app_nth1 by omega.
+    clear H2 H3.
+    generalize dependent m. generalize dependent a1.
+    induction a2; intros.
+    + destruct a1; [omega|simpl]. destruct m; reflexivity.
+    + destruct a1; [omega|simpl]. destruct m.
+      * simpl in H; omega.
+      * simpl in *. apply IHa2; omega.
+  - rewrite app_nth2 by omega.
+    rewrite app_nth2 by (simpl; omega).
+    rewrite H2 by omega.
+    replace (a2 - a1 - length [v]) with (a2 - (S a1)) by (simpl; omega).
+    clear H2 H3.
+    generalize dependent m. generalize dependent a1.
+    induction a2; intros.
+    + omega.
+    + replace (S a2 - S a1) with (a2 - a1) by omega.
+      destruct a1.
+      * replace (a2 - 0) with a2 by omega. destruct m; [simpl in *; omega|reflexivity].
+      * destruct m; [simpl in *; omega|].
+        change (skipn (S (S a1)) (w :: m)) with (skipn (S a1) m).
+        change (nth (S a2) (w :: m)) with (nth a2 m).
+        apply IHa2; simpl in *; try omega.
+Qed.
 
-Lemma write_read_half: forall sz m (a: word (S sz)) v ,
-  read_half (write_half m a v) a = v.
+Lemma write_read_half_eq: forall m a1 a2 v,
+    a1 + 1 < mem_size m ->
+    a2 = a1 ->
+    read_half (write_half m a1 v) a2 = v.
 Proof.
-  intros. unfold write_half, read_half in *.
-  rewrite (write_read_byte _ (write_byte m a (lobits 8 v)) (a ^+ $1) (hibits 8 v)).
+  intros. subst. unfold write_half, read_half in *.
+Admitted.
+(*
+  rewrite (write_read_byte_eq (write_byte m a1 (lobits 8 v))). (a1 + 1) _ (hibits 8 v)).
   assert (a ^+ $1 <> a) as Q by apply wplus_one_neq.
   rewrite (write_read_byte_diff _ a (a ^+ $1) _ (hibits 8 v) Q).
   rewrite write_read_byte.
   apply (combine_split 8 8).
 Qed.
+*)
